@prefix rdf: <http://www.w3.org/1999/02/22-rdf-syntax-ns#>.
@prefix rdfs: <http://www.w3.org/2000/01/rdf-schema#>.
@prefix ldf: <http://linkeddatafragments.org/vocab#>.
@prefix void: <http://rdfs.org/ns/void#>.
@prefix owl: <http://www.w3.org/2002/07/owl#>.

# Vocabulary

<http://linkeddatafragments.org/vocab> a owl:Ontology;
     rdfs:label "The Linked Data Fragments vocabulary"@en;
     rdfs:comment "The Linked Data Fragments vocabulary allows to describe specific subsets of a Linked Data dataset.".


# Main classes and properties

ldf:Dataset a owl:Class;
    rdfs:label "dataset"@en;
    rdfs:comment "A complete collection of Linked Data, as generated by a publisher."@en;
    rdfs:isDefinedBy <http://linkeddatafragments.org/vocab>;
    rdfs:subClassOf ldf:Fragment, void:Dataset;
    ldf:selectorType ldf:Everything.

ldf:Fragment a owl:Class;
    rdf:label "Linked Data Fragment"@en;
    rdfs:comment "A fragment consists of all elements of a dataset that match a certain selector, together with their metadata and controls to retrieve related fragments."@en;
    rdfs:isDefinedBy <http://linkeddatafragments.org/vocab>;
    rdfs:seeAlso ldf:Dataset.

ldf:FragmentClass a owl:Class;
    rdf:label "class of Linked Data Fragments"@en;
    rdfs:comment "A fragment class describes fragment instances that have specific additional properties."@en;
    rdfs:isDefinedBy <http://linkeddatafragments.org/vocab>;
    rdfs:seeAlso ldf:Fragment.

ldf:Page a owl:Class;
    rdf:label "Linked Data Fragment page"@en;
    rdfs:comment "Since fragment resources might be large, their representations do not always include all data. A page contains a specific part of a fragment's data, together with (part of) its metadata and controls."@en;
    rdfs:isDefinedBy <http://linkeddatafragments.org/vocab>;
    rdfs:seeAlso ldf:Fragment.

ldf:subFragment a rdf:Property;
    rdf:label "has subfragment"@en;
    rdfs:comment "The data in the object fragment is a subset of the data in the subject fragment."@en;
    rdfs:isDefinedBy <http://linkeddatafragments.org/vocab>;
    rdfs:subPropertyOf void:subset;
    rdfs:domain ldf:Fragment;
    rdfs:range ldf:Fragment.

ldf:subFragmentOf a rdf:Property;
    rdf:label "is a subfragment of"@en;
    rdfs:comment "The data in the subject fragment is a subset of the data in the object fragment."@en;
    rdfs:isDefinedBy <http://linkeddatafragments.org/vocab>;
    rdfs:domain ldf:Fragment;
    rdfs:range ldf:Fragment.

ldf:isAvailableAs a rdf:Property;
    rdf:label "is available as"@en;
    rdfs:comment "All fragments of the given class are available for this dataset."@en;
    rdfs:isDefinedBy <http://linkeddatafragments.org/vocab>;
    ldf:domain ldf:Dataset;
    ldf:range rdf:FragmentClass.

ldf:subFragmentClassOf a rdf:Property;
    rdf:label "is a sub-fragment-class of"@en;
    rdfs:comment "The subject fragment class is a specialization of the object fragment class, inheriting the latter's properties."@en;
    rdfs:isDefinedBy <http://linkeddatafragments.org/vocab>;
    rdfs:subPropertyOf rdfs:subClassOf;
    ldf:domain rdf:FragmentClass;
    ldf:range rdf:FragmentClass.


# Common fragment classes

ldf:BasicLdf rdfs:subClassOf ldf:Fragment;
    rdf:label "Basic Linked Data Fragment"@en;
    rdfs:comment "A Basic Linked Data Fragment has a triple pattern as selector, details count metadata, and provides controls towards any other Basic Linked Data Fragment of the same dataset."@en;
    rdfs:isDefinedBy <http://linkeddatafragments.org/vocab>;
    ldf:selectorType ldf:TriplePattern;
    ldf:providesProperty void:triples.

ldf:SubjectFragment rdfs:subClassOf ldf:Fragment;
    rdf:label "subject fragment"@en;
    rdfs:comment "A subject fragment provides data about a specific resource, typically in response to a dereferencing operation."@en;
    rdfs:isDefinedBy <http://linkeddatafragments.org/vocab>;
    ldf:selectorType ldf:SubjectPattern.

ldf:SparqlResult rdfs:subClassOf ldf:Fragment;
    rdf:label "SPARQL result"@en;
    rdfs:comment "A SPARQL result is a fragment that has a SPARQL CONSTRUCT query as its selector, typically resulting from a SPARQL endpoint response."@en;
    rdfs:isDefinedBy <http://linkeddatafragments.org/vocab>;
    ldf:selectorType ldf:SparqlQuery.


# Selector classes

ldf:Everything rdfs:subClassOf ldf:Selector;
    rdf:label "everything"@en;
    rdfs:comment "The everything selector selects all items in a dataset."@en;
    rdfs:isDefinedBy <http://linkeddatafragments.org/vocab>;
    rdfs:subClassOf ldf:BasicGraphPattern;
    ldf:hasPattern "{ ?subject ?predicate ?object }".

ldf:TriplePattern rdfs:subClassOf ldf:Selector;
    rdf:label "triple pattern"@en;
    rdfs:comment "A triple pattern selector selects all items in a dataset that match a specific triple pattern."@en;
    rdfs:isDefinedBy <http://linkeddatafragments.org/vocab>;
    rdfs:subClassOf ldf:BasicGraphPattern;
    ldf:hasPattern "{ ?subject ?predicate ?object }";
    ldf:optionalParameter "subject", "predicate", "object".

ldf:SubjectPattern rdfs:subClassOf ldf:Selector;
    rdf:label "subject pattern"@en;
    rdfs:comment "A triple pattern selector selects all items in a dataset that have a specific subject."@en;
    rdfs:isDefinedBy <http://linkeddatafragments.org/vocab>;
    rdfs:subClassOf ldf:BasicGraphPattern;
    ldf:hasPattern "{ ?subject ?predicate ?object }";
    ldf:requiredParameter "subject".

ldf:SparqlQuery rdfs:subClassOf ldf:Selector;
    rdf:label "SPARQL query"@en;
    rdfs:comment "A SPARQL query selector selects all items in a dataset that match a specific SPARQL CONSTRUCT query."@en;
    rdfs:isDefinedBy <http://linkeddatafragments.org/vocab>.

ldf:BasicGraphPattern rdfs:subClassOf ldf:Selector;
    rdf:label "basic graph pattern"@en;
    rdfs:comment "A basic graph pattern selects all items in a dataset that match a specific basic graph pattern."@en;
    rdfs:isDefinedBy <http://linkeddatafragments.org/vocab>.


# Paging

ldf:more
    rdf:label "has more data at"@en;
    rdfs:comment "This representation does not contain all data in the fragment; more can be found at the specified location."@en;
    rdfs:isDefinedBy <http://linkeddatafragments.org/vocab>;
    ldf:domain ldf:Fragment;
    # ldf:more might also be used for dumps. Does that make them pages?
    ldf:range ldf:Page.

ldf:isPageOf
    rdf:label "is a page of"@en;
    rdfs:comment "The subject is a page of the fragment."@en;
    rdfs:isDefinedBy <http://linkeddatafragments.org/vocab>;
    ldf:domain ldf:Page;
    ldf:range ldf:Fragment.
